Add example for oblivious lookup with different public view.

theories/demo/demo1.v
@@ -30,22 +30,38 @@ Notation "'succ' e" := <{ fold<nat> (inr<𝟙 + @nat> e) }>
 
 Definition is_zero : atom := "is_zero".
 Definition pred : atom := "pred".
+
 Definition otree : atom := "~tree".
 Notation "'~tree'" := (otree) (in custom oadt).
 Definition s_tree : atom := "s_tree".
 Definition r_tree : atom := "r_tree".
+
+Definition spine : atom := "spine".
+Definition otree' : atom := "~tree'".
+Notation "'~tree''" := (otree') (in custom oadt).
+Definition s_tree' : atom := "s_tree'".
+Definition r_tree' : atom := "r_tree'".
+
 Definition insert : atom := "insert".
 Definition oinsert : atom := "~insert".
 Notation "'~insert'" := (oinsert) (in custom oadt).
 Definition lookup : atom := "lookup".
 Definition olookup : atom := "~lookup".
 Notation "'~lookup'" := (olookup) (in custom oadt).
+Definition olookup' : atom := "~lookup'".
+Notation "'~lookup''" := (olookup') (in custom oadt).
 
 Notation "'leaf'" := <{ fold<tree> (inl<𝟙 + int * @tree * @tree> ()) }>
                      (in custom oadt).
 Notation "'node' e" := <{ fold<tree> (inr<𝟙 + int * @tree * @tree> e) }>
                        (in custom oadt at level 0,
                            e custom oadt at level 0).
+Notation "'sleaf'" := <{ fold<spine> (inl<𝟙 + @spine * @spine> ()) }>
+                      (in custom oadt).
+Notation "'snode' e" := <{ fold<spine> (inr<𝟙 + @spine * @spine> e) }>
+                        (in custom oadt at level 0,
+                            e custom oadt at level 0).
+
 
 (* Global definitions. *)
 Definition defs := [{
@@ -57,11 +73,8 @@ Definition defs := [{
     else 𝟙 ~+ ~int * (~tree (pred $0)) * (~tree (pred $0));
 
   (* def zero :{⊥} @nat := fold<nat> (inl<𝟙 + nat> ()); *)
-
   (* def succ :{⊥} Π:nat, nat := \:nat => fold<nat> (inr<𝟙 + nat> $0); *)
-
   (* def leaf :{⊥} @tree := fold<tree> (inl<𝟙 + int * tree * tree> ()); *)
-
   (* def node :{⊤} Π~:int * tree * tree, tree := *)
   (*   \~:int * tree * tree => fold<tree> (inr<𝟙 + int * tree * tree> $0); *)
 
@@ -101,6 +114,10 @@ Definition defs := [{
       then node (($0).1.1, insert $2 ($0).1.2, ($0).2)
       else node (($0).1.1, ($0).1.2, insert $2 ($0).2);
 
+  def ~insert :{⊥} Π:~int, Π:nat, Π:~tree $0, ~tree (succ $1) :=
+    \:~int => \:nat => \:~tree $0 =>
+      s_tree (insert (r_int $2) (r_tree $1 $0)) (succ $1);
+
   def lookup :{⊤} Π~:int, Π~:tree, 𝔹 :=
     \~:int => \~:tree =>
     case unfold<tree> $0 of
@@ -115,9 +132,39 @@ Definition defs := [{
     \:~int => \:nat => \:~tree $0 =>
       tape (s𝔹 (lookup (r_int $2) (r_tree $1 $0)));
 
-  def ~insert :{⊥} Π:~int, Π:nat, Π:~tree $0, ~tree (succ $1) :=
-    \:~int => \:nat => \:~tree $0 =>
-      s_tree (insert (r_int $2) (r_tree $1 $0)) (succ $1)
+  (* Use the upper bound of spine as public view. *)
+  data spine := 𝟙 + spine * spine;
+  obliv ~tree' (:spine) :=
+    case unfold<spine> $0 of
+      𝟙
+    | 𝟙 ~+ ~int * (~tree' ($0).1) * (~tree' ($0).2);
+  def s_tree' :{⊥} Π~:tree, Π:spine, ~tree' $0 :=
+    \~:tree => \:spine =>
+      case unfold<spine> $0 of
+        ()
+      | tape (case unfold<tree> $2 of
+                   ~inl<𝟙 ~+ ~int * (~tree' ($1).1) * (~tree' ($1).2)> ()
+                 | ~inr<𝟙 ~+ ~int * (~tree' ($1).1) * (~tree' ($1).2)>
+                     tape (s_int ($0).1.1,
+                           s_tree' ($0).1.2 ($1).1,
+                           s_tree' ($0).2 ($1).2));
+  def r_tree' :{⊤} Π:spine, Π:~tree' $0, tree :=
+    \:spine =>
+      case unfold<spine> $0 of
+        \:𝟙 => leaf
+      | \:𝟙 ~+ ~int * (~tree' ($0).1) * (~tree' ($0).2) =>
+          ~case $0 of
+            leaf
+          | node (r_int ($0).1.1,
+                  r_tree' ($2).1 ($0).1.2,
+                  r_tree' ($2).2 ($0).2);
+
+  (* An oblivious lookup function that uses [~tree'] instead. Note that the
+  implementation is basically the same as [~lookup] above with different
+  oblivious tree and its section/retraction functions. *)
+  def ~lookup' :{⊥} Π:~int, Π:spine, Π:~tree' $0, ~𝔹 :=
+    \:~int => \:spine => \:~tree' $0 =>
+      tape (s𝔹 (lookup (r_int $2) (r_tree' $1 $0)))
 }].
 
 Definition Σ : gctx := list_to_map defs.
@@ -134,6 +181,7 @@ Qed.
 
 (** Semantics. *)
 (* Warning: very slow. *)
+
 
 (* An example oblivious tree type, with index 2. *)
 Example ex_tree_type :=
@@ -246,6 +294,75 @@ Defined.
 
 Definition ex_olookup2_result := ltac:(extract ex_olookup2).
 Print ex_olookup2_result.
+
+
+(* An example of [~lookup'] which uses a different public view. *)
+Notation "'ex_spine'" := <{ snode ((snode (sleaf, sleaf)), sleaf) }>
+                         (in custom oadt, only parsing).
+
+Example ex_spine_tree_type :=
+  <{ ~tree' ex_spine }>.
+Print ex_spine_tree_type.
+
+Definition ex_spine_tree_type_pack :
+  sigT (fun ω => Σ ⊨ ex_spine_tree_type -->* ω /\ otval ω).
+Proof.
+  repeat esplit.
+  eapply mstep_alt_mstep.
+
+  repeat mstep_tac.
+
+  cbn.
+  constructor.
+  repeat step_tac.
+Defined.
+
+Definition ex_spine_tree_type_v := ltac:(extract ex_spine_tree_type_pack).
+Print ex_spine_tree_type_v.
+
+(* An example tree. *)
+Definition ex_spine_tree :=
+  <{ node (i(2), node (i(1), leaf, leaf), leaf) }>.
+Print ex_spine_tree.
+
+(* An example oblivious tree *)
+Definition ex_spine_otree :=
+  <{ s_tree' ex_spine_tree ex_spine }>.
+
+(* We can evaluate it to an oblivious value. *)
+Definition ex_spine_otree_pack :
+  sigT (fun v => Σ ⊨ ex_spine_otree -->* v /\ oval v).
+Proof.
+  repeat esplit.
+  eapply mstep_alt_mstep.
+
+  repeat mstep_tac.
+
+  cbn.
+  constructor.
+  repeat step_tac.
+Defined.
+
+Definition ex_spine_otree_v := ltac:(extract ex_spine_otree_pack).
+Print ex_spine_otree_v.
+
+(* Examples of oblivious lookup. *)
+Definition ex_spine_olookup1 :
+  sigT (fun v => Σ ⊨ <{ ~lookup' i[1] ex_spine ex_spine_otree_v }> -->* v /\ val v).
+Proof.
+  repeat esplit.
+  eapply mstep_alt_mstep.
+
+  repeat mstep_tac.
+
+  cbn.
+  constructor.
+  repeat step_tac.
+Defined.
+
+Definition ex_spine_olookup1_result := ltac:(extract ex_spine_olookup1).
+Print ex_spine_olookup1_result.
+
 
 (* An example of insert. *)
 Definition ex_insert :
